.

theories/Data/Vector.v
@@ -1,3 +1,4 @@
+Require Import Coq.Arith.PeanoNat.
 Require Import Coq.Classes.RelationClasses.
 Require Import Coq.Program.Basics.
 Require Import Coq.Relations.Relation_Definitions.
@@ -48,6 +49,166 @@ End MyFin.
 
 Module MyVec.
 
+  Import MyFin.
+
   Global Open Scope vector_scope.
+
+  Fixpoint vector_indexing {A : Type} {n : nat} (xs : vector A n) {struct xs} : Fin n -> A :=
+    match xs with
+    | [] => Fin_case0
+    | x :: xs => Fin_caseS x (vector_indexing xs)
+    end
+  .
+
+  Global Infix " !! " := vector_indexing (at level 65, left associativity) : program_scope.
+
+  Lemma vector_indexing_unfold {A : Type} {n : nat} (xs : vector A n) :
+    forall i : Fin n,
+    xs !! i =
+    match i in Fin m return vector A m -> A with
+    | @FZ n' => fun v : vector A (S n') => vector_head v
+    | @FS n' i' => fun v : vector A (S n') => vector_tail v !! i'
+    end xs.
+  Proof.
+    destruct xs as [ | n' x' xs']; [introFin0 | introFinS i'].
+    - exact (eq_reflexivity x').
+    - exact (eq_reflexivity (xs' !! i')).
+  Qed.
+
+  Global Instance vector_isSetoid (A : Hask.t) (n : nat) {requiresSetoid : isSetoid A} : isSetoid (vector A n) :=
+    { eqProp (lhs : vector A n) (rhs : vector A n) := forall i : Fin n, lhs !! i == rhs !! i
+    ; eqProp_Equivalence := equivalence_relation_by_image vector_indexing (arrow_isSetoid requiresSetoid)
+    }
+  .
+
+  Theorem vector_extensionality {A : Type} {n : nat} (xs1 : vector A n) (xs2 : vector A n)
+    (POINTWISE_EQUALITY : forall i : Fin n, xs1 !! i = xs2 !! i)
+    : xs1 = xs2.
+  Proof.
+    revert xs1 xs2 POINTWISE_EQUALITY; induction n as [ | n IH].
+    - introVNil; introVNil; intros hyp_eq.
+      exact (eq_reflexivity (@VNil A)).
+    - introVCons x1 xs1; introVCons x2 xs2; intros hyp_eq.
+      assert (x1_eq_x2 : x1 = x2) by exact (hyp_eq FZ).
+      assert (xs1_eq_xs2 : xs1 = xs2) by exact (IH xs1 xs2 (fun i : Fin n => hyp_eq (FS i))).
+      exact (eq_congruence2 (@VCons A n) x1 x2 x1_eq_x2 xs1 xs2 xs1_eq_xs2).
+  Qed.
+
+  Fixpoint vector_map {A : Type} {B : Type} {n : nat} (f : A -> B) (xs : vector A n) {struct xs} : vector B n :=
+    match xs with
+    | [] => []
+    | x :: xs => f x :: vector_map f xs
+    end
+  .
+
+  Lemma vector_map_spec {A : Type} {B : Type} {n : nat} (f : A -> B) (xs : vector A n)
+    : forall i : Fin n, f (xs !! i) = vector_map f xs !! i.
+  Proof.
+    induction xs as [ | n x xs IH]; [introFin0 | introFinS i].
+    all: rewrite vector_indexing_unfold.
+    - exact (eq_reflexivity (f x)).
+    - exact (IH i).
+  Qed.
+
+  Fixpoint diagonal {A : Type} {n : nat} {struct n} : vector (vector A n) n -> vector A n :=
+    match n with
+    | O => fun xss : vector (vector A O) O => []
+    | S n' => fun xss : vector (vector A (S n')) (S n') => vector_head (vector_head xss) :: diagonal (n := n') (vector_map vector_tail (vector_tail xss))
+    end
+  .
+
+  Lemma diagonal_spec {A : Type} {n : nat} (xss : vector (vector A n) n)
+    : forall i : Fin n, xss !! i !! i = diagonal xss !! i.
+  Proof.
+    revert xss; induction n as [ | n IH].
+    - introVNil; introFin0.
+    - introVCons xs xss; introFinS i; simpl.
+      + now rewrite vector_indexing_unfold.
+      + rewrite vector_indexing_unfold, <- IH.
+        now rewrite vector_map_spec with (f := vector_tail) (xs := xss) (i := i).
+  Qed.
+
+  Fixpoint replicate {A : Type} {n : nat} {struct n} : A -> vector A n :=
+    match n with
+    | O => fun x : A => []
+    | S n' => fun x : A => x :: replicate (n := n') x
+    end
+  .
+
+  Lemma replicate_spec {A : Type} {n : nat} (x : A)
+    : forall i : Fin n, x = replicate x !! i.
+  Proof.
+    induction n; [introFin0 | introFinS i]; simpl; eauto.
+  Qed.
+
+  Global Ltac reduce_monad_methods_of_vector :=
+    first
+    [ rewrite <- diagonal_spec
+    | rewrite <- vector_map_spec
+    | rewrite <- replicate_spec
+    ]
+  .
+
+  Section VectorIsMonad.
+
+  Variable n : nat.
+
+  Definition vec_n (X : Type) : Type := vector X n.
+
+  Global Instance vec_isMonad : isMonad vec_n :=
+    { pure {A : Type} := fun x : A => replicate x
+    ; bind {A : Type} {B : Type} := fun xs : vec_n A => fun k : A -> vec_n B => diagonal (vector_map k xs)
+    }
+  .
+
+  Local Instance vec_isSetoid1 : isSetoid1 vec_n :=
+    { liftSetoid1 {A : Type} (requiresSetoid : isSetoid A) := vector_isSetoid A n (requiresSetoid := requiresSetoid)
+    }
+  .
+
+  Global Instance vec_obeysMonadLaws
+    : LawsOfMonad vec_n (requiresSetoid1 := vec_isSetoid1) (requiresMonad := vec_isMonad).
+  Proof.
+    split; cbn; intros; (repeat reduce_monad_methods_of_vector); congruence.
+  Qed.
+
+  Local Existing Instance freeSetoidFromSetoid1.
+
+  Lemma vec_n_eqProp_iff (A : Type) (xs1 : vec_n A) (xs2 : vec_n A)
+    : xs1 == xs2 <-> xs1 = xs2.
+  Proof.
+    split; intros hyp_eq.
+    - exact (vector_extensionality xs1 xs2 hyp_eq).
+    - now rewrite hyp_eq.
+  Qed.
+
+  End VectorIsMonad.
+
+  Definition vector_zipWith {A : Type} {B : Type} {C : Type} {n : nat} (f : A -> B -> C) (xs : vec_n n A) (ys : vec_n n B) : vector C n :=
+    bind xs (fun x : A => bind ys (fun y : B => pure (f x y)))
+  .
+
+  Lemma vector_zipWith_spec {A : Type} {B : Type} {C : Type} {n : nat} (f : A -> B -> C) (xs : vector A n) (ys : vector B n)
+    : forall i : Fin n, f (xs !! i) (ys !! i) = vector_zipWith f xs ys !! i.
+  Proof.
+    cbn; intros i; (repeat reduce_monad_methods_of_vector); exact (eq_reflexivity (f (xs !! i) (ys !! i))).
+  Qed.
+
+  Fixpoint vector_range {n : nat} {struct n} : nat -> vector nat n :=
+    match n with
+    | O => fun m : nat => []
+    | S n' => fun m : nat => m :: vector_range (n := n') (S m)
+    end
+  .
+
+  Lemma vector_range_spec {n : nat} (m : nat)
+    : forall i : Fin n, evalFin i + m = vector_range m !! i.
+  Proof.
+    revert m; induction n as [ | n IH]; intros m; [introFin0 | introFinS i].
+    - reflexivity.
+    - rewrite evalFin_unfold; simpl.
+      rewrite <- IH with (m := S m) (i := i).
+      apply Nat.add_succ_comm.
+  Qed.
 
 End MyVec.
